isim rules

proofmode/IProofMode.v
@@ -92,13 +92,18 @@ Section SIM.
   (* Variable stb_src: gname -> fspec.
   Variable stb_tgt: gname -> fspec. *)
 
+  Definition quantify_ctx (P: Σ -> Σ -> Prop) : Σ -> Prop:=
+    fun fmr => forall ctx (WF: URA.wf (fmr ⋅ ctx)), P ctx fmr.
+
+  Definition ignore_ctx {X} {Y} (P: X -> Y -> iProp) : X -> Y -> Σ -> iProp :=
+    fun x y _ => P x y.
+
   Program Definition isim
           r g {R} (RR: Any.t * R-> Any.t * R -> iProp) ps pt
           (sti_src sti_tgt : Any.t * itree hAGEs R): iProp :=
-    iProp_intro (fun fmr => forall ctx (WF: URA.wf (fmr ⋅ ctx)),
-                            gpaco8 (_hpsim) (cpn8 _hpsim) r g R (RR ps pt sti_src sti_tgt ctx fmr) _.
+    iProp_intro (quantify_ctx (gpaco8 (_hpsim) (cpn8 _hpsim) r g R (ignore_ctx RR) ps pt sti_src sti_tgt)) _.
   Next Obligation.
-    s. i. guclo hpsim_extendC_spec. econs; et. eapply H.
+    unfold quantify_ctx. s. i. guclo hpsim_extendC_spec. econs; et. eapply H.
     eapply URA.wf_extends; eauto.
     eapply URA.extends_add; eauto.
   Qed.
@@ -114,12 +119,12 @@ Section SIM.
       (CUR: Own fmr ⊢ #=> iP)
       (WF: URA.wf (fmr ⋅ ctx))
     :
-      gpaco8 _hpsim (cpn8 _hpsim) r g R RR ps pt (st_src, i_src) (st_tgt, i_tgt) ctx fmr.
+      gpaco8 _hpsim (cpn8 _hpsim) r g R (ignore_ctx RR) ps pt (st_src, i_src) (st_tgt, i_tgt) ctx fmr.
   Proof. Admitted.
 
   Lemma isim_final
       r g ps pt {R} RR st_src st_tgt i_src i_tgt iP fmr
-      (SIM: forall ctx (WF: URA.wf (fmr ⋅ ctx)),  gpaco8 _hpsim (cpn8 _hpsim) r g R RR ps pt (st_src, i_src) (st_tgt, i_tgt) ctx fmr)
+      (SIM: forall ctx (WF: URA.wf (fmr ⋅ ctx)),  gpaco8 _hpsim (cpn8 _hpsim) r g R (ignore_ctx RR) ps pt (st_src, i_src) (st_tgt, i_tgt) ctx fmr)
     :
       bi_entails
         iP
@@ -131,7 +136,7 @@ Section SIM.
       (CUR: Own fmr ⊢ #=> @isim r g R RR ps pt (st_src, i_src) (st_tgt, i_tgt))
       (WF: URA.wf (fmr ⋅ ctx))
     :
-      gpaco8 _hpsim (cpn8 _hpsim) r g R RR ps pt (st_src, i_src) (st_tgt, i_tgt) ctx fmr.
+      gpaco8 _hpsim (cpn8 _hpsim) r g R (ignore_ctx RR) ps pt (st_src, i_src) (st_tgt, i_tgt) ctx fmr.
   Proof. Admitted.
 
   (* Lemma isim_upd *)
@@ -182,15 +187,36 @@ Section SIM.
 
   Lemma isim_call 
     r g ps pt {R} RR st_src st_tgt k_src k_tgt fn varg
-    (* (INV: fmr ⊢ #=> (I st_src st_tgt ** FR))
-    (K: forall st_src0 st_tgt0 vret,   
-              ((I st_src0 st_tgt0 ** FR) ⊢ @isim r g R RR true true (st_src0, k_src vret) (st_tgt0, k_tgt vret))) *)
   :
   bi_entails
-    ((Ist st_src st_tgt) ** (∀ st_src0 st_tgt0 vret, (Ist st_src0 st_tgt0) -* @isim r g R RR true true (st_src0, k_src vret) (st_tgt0, k_tgt vret)))
+    (#=> (Ist st_src st_tgt ** (∀ st_src0 st_tgt0 vret, (Ist st_src0 st_tgt0) -* @isim r g R RR true true (st_src0, k_src vret) (st_tgt0, k_tgt vret))))
     (isim r g RR ps pt (st_src, trigger (Call fn varg) >>= k_src) (st_tgt, trigger (Call fn varg) >>= k_tgt)).
-    (* fmr ⊢ isim r g RR ps pt (st_src, trigger (Call fn varg) >>= k_src) (st_tgt, trigger (Call fn varg) >>= k_tgt). *)
-  Proof. Admitted.
+  Proof.
+    uipropall. unfold quantify_ctx. i.
+    edestruct (H _ WF0); des. subst. clear H.
+    guclo hpsimC_spec. econs; cycle 2.
+    { instantiate (1:= Own b). i.
+      assert (WFfmr': URA.wf fmr').
+      { eapply URA.wf_mon; eauto. }
+      uipropall. edestruct INV; try refl; eauto; des; subst.
+      guclo hpsim_extendC_spec. econs; eauto.
+      { rewrite (URA.add_comm x b0) in WF1.
+        rr in H3. uipropall. specialize (H3 st_src0).
+        rr in H3. uipropall. specialize (H3 st_tgt0).
+        rr in H3. uipropall. specialize (H3 vret).
+        uipropall. eapply H3; cycle 1.
+        { eapply H1. }
+        { eapply URA.wf_extends, WF1. repeat eapply URA.extends_add. eauto. }
+        { eapply URA.wf_mon in WF1.
+          eapply URA.wf_extends, WF1. repeat eapply URA.extends_add. eauto. }
+      }
+      { rewrite (URA.add_comm x b0). repeat eapply URA.extends_add. eauto. }
+    }
+    { apply H0. }
+    { uipropall. i. rr in H. des. subst.
+      exists a, (b ⋅ ctx0). esplits; r_solve; rr; eauto.
+    }
+  Qed.
 
   Lemma isim_syscall
     r g ps pt {R} RR st_src st_tgt k_src k_tgt fn varg rvs
@@ -296,28 +322,80 @@ Section SIM.
     (iP -* (@isim r g R RR true pt (st_src, k_src tt) (st_tgt, i_tgt)))
     (@isim r g R RR ps pt (st_src, trigger (Assume iP) >>= k_src) (st_tgt, i_tgt)).
   Proof.
-    uiprop. i. guclo hpsimC_spec. econs; i.
-    { iIntros "H". eauto. }
-    eapply iProp_sepconj in NEW; cycle 1; try refl.
-    { instantiate (1:=ε). r_solve. eauto. }
-    des. uiprop in NEW1. destruct NEW1. subst.
-    exploit (H a); eauto.
-    { revert NEW. r_solve. i. apply URA.wf_mon in NEW.
-      eapply eq_ind; eauto. r_solve. }
-    i. 
+    uiprop. unfold quantify_ctx. i. guclo hpsimC_spec. econs; i; eauto.
+    uiprop in NEW. edestruct (NEW fmr'); eauto 10; try refl.
+    { eapply URA.wf_mon; eauto. }
+    des. subst. exploit (H x); eauto; cycle 2.
+    { i. guclo hpsim_extendC_spec. econs; eauto.
+      { rewrite (URA.add_comm x b). eapply URA.extends_add; eauto. }
+      eapply URA.wf_mon. eauto.
+    }
+    { eapply URA.wf_extends, WF1. rewrite (URA.add_comm x b).
+      etrans.
+      - eapply URA.extends_add; eauto.
+      - rr; eauto.
+    }
+    { eapply URA.wf_extends, WF1.
+      rewrite (URA.add_comm x b).
+      repeat eapply URA.extends_add. eauto.
+    }
+  Qed.
 
-    
-    
-    guclo hpsim_extendC_spec. econs. eapply H.
+  Lemma isim_guarantee_src
+    r g ps pt {R} RR iP st_src st_tgt k_src i_tgt 
+  :
+  bi_entails
+    (#=> (iP ** (@isim r g R RR true pt (st_src, k_src tt) (st_tgt, i_tgt))))
+    (@isim r g R RR ps pt (st_src, trigger (Guarantee iP) >>= k_src) (st_tgt, i_tgt)).
+  Proof.
+    uiprop. unfold quantify_ctx. i.
+    edestruct (H _ WF0); des. subst.
+    guclo hpsimC_spec. econs; cycle 2.
+    { instantiate (1:= Own b). i.
+      assert (WFfmr': URA.wf fmr').
+      { eapply URA.wf_mon; eauto. }
+      assert (EXT: URA.extends b fmr').
+      { uiprop in NEW. eapply NEW; try refl; eauto. }
+      guclo hpsim_extendC_spec. econs; eauto.
+      eapply H3. eapply URA.wf_extends, WF1.
+      eapply URA.extends_add; eauto.
+    }
+    { eauto. }
+    { uiprop. i. rr in H1. des.
+      exists a, (b ⋅ ctx0). subst. r_solve.
+      esplits; eauto. rr; eauto.
+    }
+  Qed.
 
-    
-    
-    uiprop in NEW. edestruct (NEW fmr0); eauto; try refl.
-    { instantiate (1:= ε). r_solve. eauto. }
-    des. subst. exploit H; eauto. { admit. }
-    i.
-  Admitted.
+  
+  Lemma isim_guarantee_src
+    r g ps pt {R} RR iP st_src st_tgt k_src i_tgt 
+  :
+  bi_entails
+    ((#=>iP) ** (@isim r g R RR true pt (st_src, k_src tt) (st_tgt, i_tgt)))
+    (@isim r g R RR ps pt (st_src, trigger (Guarantee iP) >>= k_src) (st_tgt, i_tgt)).
+  Proof.
+    uiprop. unfold quantify_ctx. i. des. subst.
+    edestruct (H0 (b ⋅ ctx)); des.
+    { r_solve. eauto. }
+    guclo hpsimC_spec. econs; cycle 2.
+    { instantiate (1:= Own b). i.
+      assert (WFfmr': URA.wf fmr').
+      { eapply URA.wf_mon; eauto. }
+      assert (EXT: URA.extends b fmr').
+      { uiprop in NEW. eapply NEW; try refl; eauto. }
+      guclo hpsim_extendC_spec. econs; eauto.
+      eapply H1. eapply URA.wf_extends, WF1.
+      eapply URA.extends_add; eauto.
+    }
+    { revert H. r_solve. eauto. }
+    { uiprop. i. rr in H3. des.
+      exists x, (b ⋅ ctx0). subst. r_solve.
+      esplits; eauto. rr; eauto.
+    }
+  Qed.
 
+  
   Lemma isim_assume_tgt
     r g ps pt {R} RR iP st_src st_tgt i_src k_tgt 
   :
@@ -326,13 +404,6 @@ Section SIM.
     (@isim r g R RR ps pt (st_src, i_src) (st_tgt, trigger (Assume iP) >>= k_tgt)).
   Proof. Admitted.
     
-  Lemma isim_guarantee_src
-    r g ps pt {R} RR iP st_src st_tgt k_src i_tgt 
-  :
-  bi_entails
-    (iP ** (@isim r g R RR true pt (st_src, k_src tt) (st_tgt, i_tgt)))
-    (@isim r g R RR ps pt (st_src, trigger (Guarantee iP) >>= k_src) (st_tgt, i_tgt)).
-  Proof. Admitted.
 
   Lemma isim_guarantee_tgt
     r g ps pt {R} RR iP st_src st_tgt i_src k_tgt 
